tests/defined/duff.c
@@ -1,0 +1,23 @@
+#include<stdio.h>
+
+void duffs_device(unsigned char *from, unsigned char *to, int count) {
+  int n = (count + 7) / 8;
+  switch(count % 8) {
+    case 0: do { *to++ = *from++;
+    case 7: *to++ = *from++;
+    case 6: *to++ = *from++;
+    case 5: *to++ = *from++;
+    case 4: *to++ = *from++;
+    case 3: *to++ = *from++;
+    case 2: *to++ = *from++;
+    case 1: *to++ = *from++;
+               } while(--n > 0);
+  }
+}
+
+int main() {
+  long long a[10], b[10];
+  for (int i = 0; i < 10; i++) a[i] = i;
+  duffs_device((unsigned char*)a, (unsigned char*)b, sizeof(a));
+  for (int i = 0; i < 10; i++) printf("%d\n", b[i]);
+}
